GraphUtils.thy
@@ -41,7 +41,7 @@ end
 
 
 definition empty_graph :: "_ graph" where "empty_graph \<equiv> \<lambda>_. 0" (* TODO is there a better way to define constant functions? *)
-interpretation empty: Graph empty_graph .
+(*interpretation empty: Graph empty_graph .*)
 
 section \<open>Custom induction rules\<close>
 (* TODO check which of these are useful and prettify proofs *)
